save

proofmode/HPSimFacts.v
@@ -33,26 +33,63 @@ Section HPSIM.
   Variable fl_tgt: alist gname (Any.t -> itree hAGEs Any.t).
   Variable I: Any.t -> Any.t -> iProp.
 
+  Definition hp_reconf_eq cr : relation (Any.t * iProp) :=
+    fun '(str,fr) '(str',fr') =>
+      <<RELr: fr ⊢ #=> (fr' ** cr)>> /\      
+      <<STR: str' = str>>.
 
+  (* 
   Definition hp_reconf_eq cr : relation (Any.t * Σ) :=
     fun '(str,fr) '(str',fr') =>
       <<RELr: Own fr ⊢ #=> Own (fr' ⋅ cr)>> /\      
-      <<STR: str' = str>>.
-  
-  Definition hp_reconf_equiv cr : relation (Any.t * Σ) :=
+      <<STR: str' = str>>. *)    
+      
+  Definition hp_reconf_equiv cr : relation (Any.t * iProp) :=
+    fun '(str,fr) '(str',fr') =>
+      hp_reconf_eq cr (str,fr) (str',fr')
+      \/
+      (exists st (mr mr': iProp),
+       <<RELr: (fr ** mr) ⊢ #=> (fr' ** mr' ** cr)>> /\
+       <<STR: str = Any.pair st mr↑>> /\
+       <<STR': str' = Any.pair st mr'↑>>).
+
+(*  Definition hp_reconf_equiv cr : relation (Any.t * Σ) :=
     fun '(str,fr) '(str',fr') =>
       hp_reconf_eq cr (str,fr) (str',fr')
       \/
       (exists st (mr mr': Σ),
        <<RELr: Own (fr ⋅ mr) ⊢ #=> Own (fr' ⋅ mr' ⋅ cr)>> /\
        <<STR: str = Any.pair st mr↑>> /\
-       <<STR': str' = Any.pair st mr'↑>>).
+       <<STR': str' = Any.pair st mr'↑>>). *)
 
-  Definition hp_reconf_rel R (eqv: Σ -> _) cr : relation (Any.t * (Σ * R)) :=
+  Definition hp_reconf_rel R (eqv: iProp -> _) cr : relation (Any.t * (iProp * R)) :=
     fun '(str,(fr,x)) '(str',(fr',x')) =>
       eqv cr (str,fr) (str',fr') /\ x = x'.
 
+  (* Definition hp_reconf_rel R (eqv: Σ -> _) cr : relation (Any.t * (Σ * R)) :=
+    fun '(str,(fr,x)) '(str',(fr',x')) =>
+      eqv cr (str,fr) (str',fr') /\ x = x'. *)
+
   Lemma hp_reconf_equiv_strong
+    cr str str' (fr fr': iProp)
+    (EQV: hp_reconf_equiv cr (str,fr) (str',fr'))
+    :
+    (hp_reconf_eq cr (str,fr) (str',fr') /\
+     <<FAIL: ~ exists st (mr:iProp), str = Any.pair st mr↑>>)
+    \/
+    (exists st (mr mr': iProp),
+     <<RELr: (fr ** mr) ⊢ #=> (fr' ** mr' ** cr)>> /\
+     <<STR: str = Any.pair st mr↑>> /\
+     <<STR': str' = Any.pair st mr'↑>>).
+  Proof.
+    ss. des; subst; [|right]; esplits; eauto.
+    destruct (classic (exists stx (mrx:iProp), str = Any.pair stx mrx↑)); eauto.
+    des. subst. right. esplits; eauto.
+    iIntros "[H H0]". iPoseProof (RELr with "H") as "H". iMod "H". iModIntro.
+    iFrame. iFrame.
+  Qed.
+  
+  (* Lemma hp_reconf_equiv_strong
     cr str str' (fr fr': Σ)
     (EQV: hp_reconf_equiv cr (str,fr) (str',fr'))
     :
@@ -70,8 +107,27 @@ Section HPSIM.
     eapply own_ctx with (ctx := mrx) in RELr. revert RELr. r_solve. i.
     rewrite-> URA.add_comm, (URA.add_comm fr' mrx). eauto.
   Qed.
-  
+   *)
+
   Lemma hp_reconf_fail
+    r R RR str i i'
+    (FAIL: ~ exists st (mr:iProp), str = Any.pair st mr↑)
+    :
+    paco4 _sim_strict r R RR
+      (str, p <- unwrapU (Any.split str);;
+            mr <- (let '(st,_mr) := p in unwrapU (@Any.downcast iProp _mr));; i mr)
+      (str, p <- unwrapU (Any.split str);;
+            mr <- (let '(st,_mr) := p in unwrapU (@Any.downcast iProp _mr));; i' mr).
+  Proof.
+    destruct (Any.split str) eqn:STR; cycle 1.
+    { ss. unfold triggerUB. grind. pstep. econs. i. inv x. }
+    grind. destruct (Any.downcast t0) eqn:T0; cycle 1.
+    { ss. unfold triggerUB. grind. pstep. econs. i. inv x. }
+    apply Any.split_pair in STR. apply Any.downcast_upcast in T0.
+    exfalso. eapply FAIL. des; subst. eauto.
+  Qed.
+
+  (* Lemma hp_reconf_fail
     r R RR str i i'
     (FAIL: ~ exists st (mr:Σ), str = Any.pair st mr↑)
     :
@@ -87,9 +143,34 @@ Section HPSIM.
     { ss. unfold triggerUB. grind. pstep. econs. i. inv x. }
     apply Any.split_pair in STR. apply Any.downcast_upcast in T0.
     exfalso. eapply FAIL. des; subst. eauto.
-  Qed.
+  Qed. *)
 
-  Lemma handle_Guarantee_reconf
+  (* Lemma handle_Guarantee_reconf
+    P str str' (fr fr' cr: iProp)
+    (RELr: hp_reconf_equiv cr (str,fr) (str',fr'))
+    :
+    sim_strict _ (hp_reconf_rel _ hp_reconf_equiv cr)
+      (str, handle_Guarantee P fr)
+      (str', handle_Guarantee P fr').
+  Proof.
+    ginit. unfold handle_Guarantee, guarantee, mget, mput.
+    grind; gstep; econs; i. destruct x' as [[c0 c1] c2]. exists (c0, c1, c2⋅cr).
+    grind; gstep; econs; i.
+    grind; apply hp_reconf_equiv_strong in RELr; repeat (rr in RELr; des; subst).
+    { gfinal. right. apply hp_reconf_fail. eauto. }
+    rewrite !Any.pair_split. grind. rewrite !Any.upcast_downcast.
+    grind; gstep; econs; i. eexists.
+    { r_solve. iIntros "H". iPoseProof (RELr0 with "H") as "H". iMod "H".
+      iDestruct "H" as "[X Y]". iSplitL "X"; eauto.
+      iPoseProof (x' with "X") as "X". eauto. }
+    grind; gstep; econs; i. eexists. { eauto. }
+    grind; gstep; econs; i. grind. rewrite !Any.pair_split.
+    repeat (grind; gstep; econs; i).
+    split; eauto. right. esplits; eauto.
+    r_solve. eauto.
+  Qed. *)
+
+  (* Lemma handle_Guarantee_reconf
     P str str' (fr fr' cr: Σ)
     (RELr: hp_reconf_equiv cr (str,fr) (str',fr'))
     :
@@ -112,9 +193,9 @@ Section HPSIM.
     repeat (grind; gstep; econs; i).
     split; eauto. right. esplits; eauto.
     r_solve. eauto.
-  Qed.
+  Qed. *)
 
-  Lemma handle_Guarantee_reconf_true
+  (* Lemma handle_Guarantee_reconf_true
     str str' (fr fr' cr: Σ)
     (RELr: hp_reconf_equiv cr (str,fr) (str',fr'))
     :
@@ -137,8 +218,33 @@ Section HPSIM.
     grind; gstep; econs; i. grind. rewrite !Any.pair_split.
     repeat (grind; gstep; econs; i).
     split; eauto. split; eauto.
-  Qed.
+  Qed. *)
 
+  (* Lemma handle_Guarantee_reconf_true
+    str str' (fr fr' cr: Σ)
+    (RELr: hp_reconf_equiv cr (str,fr) (str',fr'))
+    :
+    sim_strict _ (hp_reconf_rel _ hp_reconf_eq cr)
+      (str, handle_Guarantee True fr)
+      (str', handle_Guarantee True fr').
+  Proof.
+    ginit. unfold handle_Guarantee, guarantee, mget, mput.
+    grind; gstep; econs; i. destruct x' as [[c0 c1] c2]. exists (c0, c1⋅cr, c2).
+    grind; gstep; econs; i.
+    grind; apply hp_reconf_equiv_strong in RELr; repeat (rr in RELr; des; subst).
+    { gfinal. right. apply hp_reconf_fail. eauto. }
+    rewrite !Any.pair_split. grind. rewrite !Any.upcast_downcast.
+    grind; gstep; econs; i. eexists.
+    { r_solve. iIntros "H". iPoseProof (RELr0 with "H") as "H". iMod "H".
+      iDestruct "H" as "[X Y]".
+      rewrite -URA.add_assoc (URA.add_comm cr c2) URA.add_assoc.
+      iSplitL "X"; eauto. iPoseProof (x' with "X") as "X". eauto. }
+    grind; gstep; econs; i. eexists. { eauto. }
+    grind; gstep; econs; i. grind. rewrite !Any.pair_split.
+    repeat (grind; gstep; econs; i).
+    split; eauto. split; eauto.
+  Qed.  *)
+(* 
   Lemma trigger_hAGE_simpl R (P: iProp) (e : hAGE R):
     (trigger (e|)%sum : itree hAGEs R) = trigger e.
   Proof. reflexivity. Qed.
@@ -308,7 +414,7 @@ Section HPSIM.
       r in REL1. des; subst. eauto. }
     i. gstep; econs. rr in REL1. des; subst.
     destruct v0, v0'. s in REL2; des; subst. eauto. 
-  Qed.
+  Qed. *)
 
 
   (*** ****)
@@ -318,7 +424,17 @@ Section HPSIM.
 
 
 
-Variant interp_inv: Σ -> Any.t * Any.t -> Prop :=
+Variant interp_inv: iProp -> Any.t * Any.t -> Prop :=
+| interp_inv_intro
+    (ctx mr_src mr_tgt: iProp) st_src st_tgt mr
+    (SRC: ⊢ #=> mr_src)
+    (MRS: mr_src ⊢ #=> (ctx ** mr ** mr_tgt))
+    (MR: mr ⊢ #=> I st_src st_tgt)
+  :
+  interp_inv ctx (Any.pair st_src mr_src↑, Any.pair st_tgt mr_tgt↑)
+.
+
+(* Variant interp_inv: Σ -> Any.t * Any.t -> Prop :=
 | interp_inv_intro
     (ctx mr_src mr_tgt: Σ) st_src st_tgt mr
     (WF: URA.wf mr_src)
@@ -326,10 +442,173 @@ Variant interp_inv: Σ -> Any.t * Any.t -> Prop :=
     (MR: Own mr ⊢ #=> I st_src st_tgt)
   :
   interp_inv ctx (Any.pair st_src mr_src↑, Any.pair st_tgt mr_tgt↑)
-.
+. *)
 
 
 
+(* remove later *)
+Tactic Notation "uiprop" := repeat (autounfold with iprop; autorewrite with iprop; s).
+Tactic Notation "uiprop" "in" hyp(H)  := repeat (autounfold with iprop in H; autorewrite with iprop in H; simpl in H).
+
+Program Definition isim_body
+p_src p_tgt
+(sti_src sti_tgt : Any.t * itree hAGEs Any.t): iProp := 
+iProp_intro (hpsim_body fl_src fl_tgt I p_src p_tgt sti_src sti_tgt) _.
+Next Obligation.
+  Admitted.
+  (* guclo hpsim_extendC_spec. econs; et.
+Qed. *)
+
+
+Lemma hpsim_adequacy:
+forall
+  (fl_src0 fl_tgt0: alist string (Any.t -> itree Es Any.t)) 
+  (FLS: fl_src0 = List.map (fun '(s, f) => (s, interp_hp_fun f)) fl_src)
+  (FLT: fl_tgt0 = List.map (fun '(s, f) => (s, interp_hp_fun f)) fl_tgt)
+  p_src p_tgt st_src st_tgt itr_src itr_tgt fmrP
+  (ctx mr_src mr_tgt fr_src fr_tgt: iProp)
+  (SIM: fmrP = isim_body p_src p_tgt (st_src, itr_src) (st_tgt, itr_tgt))
+  (SRC: ⊢ #=> (fr_src ** mr_src))
+  (FMR: fr_src ** mr_src ⊢ #=> (ctx ** fmrP ** (fr_tgt ** mr_tgt))),
+@sim_itree iProp interp_inv eq fl_src0 fl_tgt0 p_src p_tgt ctx
+  (Any.pair st_src mr_src↑, interp_hp_body itr_src fr_src)
+  (Any.pair st_tgt mr_tgt↑, interp_hp_body itr_tgt fr_tgt).
+Proof.
+i. apply hpsim_add_dummy in SIM.
+revert_until I. ginit. gcofix CIH. i.
+remember (st_src, itr_src). remember (st_tgt, itr_tgt).
+move SIM before FLT. revert_until SIM.
+punfold SIM. induction SIM; i; clarify; cycle 1.
+- unfold interp_hp_body. 
+steps. unfold handle_Guarantee, guarantee, mget, mput. steps_safe.
+force_l. instantiate (1:= (⌜True⌝%I, ctx ** b ** b0 ** (I st_src0 st_tgt0) ** FR)). steps_safe.
+force_l.
+{
+  iIntros "H". iPoseProof (FMR0 with "H") as "H". iMod "H". iDestruct "H" as "[[H H0] H1]".
+  iPoseProof (x with "H1") as "H1". iMod "H1".
+  iPoseProof (INV with "H0") as "H0". iMod "H0".
+  iDestruct "H1" as "[[_ H1] H2]". iFrame. iFrame. et. 
+}
+steps_safe. 
+force_l; et.
+steps_safe. eapply safe_sim_sim; econs. esplits; i.
+{ econs; cycle 2. 
+  { instantiate (1:= I st_src0 st_tgt0). et. } 
+  { iIntros. iPoseProof SRC as "H".
+    iPoseProof (FMR0 with "H") as "H0".
+    admit. 
+  }
+  { instantiate (1:= ctx ** FR ** b). iIntros "[[[[H H0] H1] H2] H3]". iFrame. et. }
+}
+steps.
+inv WF0. eapply H. [eapply WF| |et|et|r_solve; et| |].
+{ eapply H0. }
+{  
+  eapply own_wf in MRS; et.
+  replace (ctx ⋅ fr ⋅ frt ⋅ mr0 ⋅ mr_tgt0) with (fr ⋅ mr0 ⋅ (ctx ⋅ frt ⋅ mr_tgt0)) in MRS; r_solve.
+  eapply URA.wf_mon; et.
+}
+{
+  iIntros "[H H0]". 
+  iPoseProof (H2 with "H") as "FR". iPoseProof (MR with "H0") as "INV". iMod "INV".  
+  iFrame. et.
+}
+{ r_solve. replace (ctx ⋅ fr ⋅ mr0 ⋅ frt ⋅ mr_tgt0) with (ctx ⋅ fr ⋅ frt ⋅ mr0 ⋅ mr_tgt0); et. r_solve. }
+
+
+
+
+
+Lemma hpsim_adequacy:
+forall
+  (fl_src0 fl_tgt0: alist string (Any.t -> itree Es Any.t)) 
+  (FLS: fl_src0 = List.map (fun '(s, f) => (s, interp_hp_fun f)) fl_src)
+  (FLT: fl_tgt0 = List.map (fun '(s, f) => (s, interp_hp_fun f)) fl_tgt)
+  p_src p_tgt st_src st_tgt itr_src itr_tgt fmr
+  (ctx mr_src mr_tgt fr_src fr_tgt: iProp)
+  (SIM: hpsim_body fl_src fl_tgt I p_src p_tgt (st_src, itr_src) (st_tgt, itr_tgt) fmr)
+  (WF: URA.wf fmr)
+  (SRC: ⊢ #=> (fr_src ** mr_src))
+  (FMR: fr_src ** mr_src ⊢ #=> (ctx ** (Own fmr) ** (fr_tgt ** mr_tgt))),
+@sim_itree iProp interp_inv eq fl_src0 fl_tgt0 p_src p_tgt ctx
+  (Any.pair st_src mr_src↑, interp_hp_body itr_src fr_src)
+  (Any.pair st_tgt mr_tgt↑, interp_hp_body itr_tgt fr_tgt).
+Proof.
+i. apply hpsim_add_dummy in SIM.
+revert_until I. ginit. gcofix CIH. i.
+remember (st_src, itr_src). remember (st_tgt, itr_tgt).
+move SIM before FLT. revert_until SIM.
+punfold SIM. induction SIM; i; clarify.
+- unfold interp_hp_body, hp_fun_tail, handle_Guarantee, guarantee, mget, mput.
+  steps. force_l. instantiate (1 := (b, ctx ** (Own fmr) ** b0)). steps.
+  force_l.
+  { iIntros "H". iPoseProof (FMR with "H") as "H". iMod "H".
+    admit.  
+  } 
+  steps. force_l; et. 
+  steps. econs.
+  unfold hpsim_end in RET.
+  esplits; et.
+  { 
+    econs; et.
+    {
+      iIntros. iPoseProof SRC as "H". iMod "H". admit.  
+    }
+    { iIntros "H". iPoseProof (RET with "H") as "H". iMod "H". iDestruct "H" as "[H H0]". et. }
+  }
+  {
+    rr in RET. uiprop in RET. hexploit RET; [et|refl|instantiate (1:= ε); r_solve; et|].
+    i. des. rr in H2. uipropall.
+  }
+- unfold interp_hp_body. hexploit INV. i.
+  steps. unfold handle_Guarantee, guarantee, mget, mput. steps_safe.
+  force_l. instantiate (1:= (⌜True⌝%I, ctx ** b ** b0 ** (I st_src0 st_tgt0) ** FR)). steps_safe.
+  force_l.
+  {
+    iIntros "H". iPoseProof (FMR with "H") as "H". iMod "H". iDestruct "H" as "[[H H0] H1]".
+    iPoseProof (x with "H1") as "H1". iMod "H1".
+    iPoseProof (H0 with "H0") as "H0". iMod "H0".
+    iDestruct "H1" as "[[_ H1] H2]". iFrame. iFrame. et. 
+  }
+  steps_safe. 
+  force_l; et.
+  steps_safe. eapply safe_sim_sim; econs. esplits; i.
+  { econs; cycle 2. 
+    { instantiate (1:= I st_src0 st_tgt0). et. } 
+    { iIntros. iPoseProof SRC as "H".
+      iPoseProof (FMR with "H") as "H0".
+      admit. 
+    }
+    { instantiate (1:= ctx ** FR ** b). iIntros "[[[[H H0] H1] H2] H3]". iFrame. et. }
+  }
+  steps.
+  inv WF0. eapply H. [eapply WF| |et|et|r_solve; et| |].
+  { eapply H0. }
+  {  
+    eapply own_wf in MRS; et.
+    replace (ctx ⋅ fr ⋅ frt ⋅ mr0 ⋅ mr_tgt0) with (fr ⋅ mr0 ⋅ (ctx ⋅ frt ⋅ mr_tgt0)) in MRS; r_solve.
+    eapply URA.wf_mon; et.
+  }
+  {
+    iIntros "[H H0]". 
+    iPoseProof (H2 with "H") as "FR". iPoseProof (MR with "H0") as "INV". iMod "INV".  
+    iFrame. et.
+  }
+  { r_solve. replace (ctx ⋅ fr ⋅ mr0 ⋅ frt ⋅ mr_tgt0) with (ctx ⋅ fr ⋅ frt ⋅ mr0 ⋅ mr_tgt0); et. r_solve. }
+
+
+
+
+
+
+
+
+
+
+
+
+
+(* 
 Lemma hpsim_adequacy:
 forall
   (fl_src0 fl_tgt0: alist string (Any.t -> itree Es Any.t)) 
@@ -546,6 +825,6 @@ punfold SIM. induction SIM; i; clarify.
     rewrite <- URA.add_assoc. eapply own_ctx. et.
   }
 - pclearbot. gstep. econs. gfinal. left. eapply CIH; et.
-Qed.
+Qed. *)
 
 End HPSIM.
